commit

Snoclist.v
@@ -1,10 +1,11 @@
+Require Import Arith.
 
-Inductive snoclist (A : Type) : Type :=
-| nil : snoclist A
-| snoc : snoclist A -> A -> snoclist A.
+Inductive snoclist (A : Type) : nat -> Type :=
+| nil : snoclist A 0
+| snoc : forall n : nat, snoclist A n -> A -> snoclist A (S n).
 
 Arguments nil {A}.
-Arguments snoc {A} l a.
+Arguments snoc {A} {n} l a.
 
 Declare Scope snoclist_scope.
 Delimit Scope snoclist_scope with snoclist.
@@ -25,19 +26,16 @@ End SnoclistNotations.
 
 Import SnoclistNotations.
 
-Definition length {A : Type} : snoclist A -> nat :=
-  fix length l :=
-  match l with
-   | nil => O
-   | l' :: _ => S (length l')
-  end.
+(*Definition length {A : Type} {n : nat} : snoclist A n -> nat := fix length l := n.*)
 
-Definition app {A : Type} : snoclist A -> snoclist A -> snoclist A :=
-  fix app l m :=
-  match m with
-   | nil => l
-   | m' :: a => app l m' :: a
-  end.
+Theorem snoclist_comm {A : Type} {n m : nat} : snoclist A (m + n) -> snoclist A (n + m).
+Proof. rewrite Nat.add_comm. intro h. apply h. Qed.
+
+Fixpoint app {A : Type} {n m : nat} (l : snoclist A n) (r : snoclist A m) : snoclist A (n + m) :=
+match r in (snoclist _ m) return (snoclist _ (m + n) -> snoclist _ (n + m)) -> snoclist _ (n + m) with
+| nil => fun H => H l
+| r' :: a => fun H => H ( snoclist_comm (app l r') :: a)
+end snoclist_comm.
 
 Infix "++" := app (right associativity, at level 60) : snoclist_scope.
 
@@ -45,7 +43,11 @@ Section Facts.
 
 Variable A : Type.
 
+(*
 Theorem nil_snoc (x:A) (l:snoclist A) : [] <> l :: x.
-Admitted.
+Proof.
+discriminate.
+Qed.
+*)
 
 End Facts.
