Workbench.v
@@ -1,20 +1,113 @@
-
+Require Import Nat.
 Require Import Snoclist.
 Import SnoclistNotations.
 Require Import PlanarLambda.
 Require Import Types.
 
-Definition context : Type := snoclist type.
+Require List.
 
-Inductive test (n : nat) (pt : pterm n) : Type :=
-| Test : test n pt.
+Definition context n : Type := snoclist type n.
 
-Inductive test2 : nat -> Type :=
-| Test2 : test2 0.
+Inductive is_typed : forall {a : nat}, context a -> pterm a -> type -> Prop :=
+| typed_var ty : is_typed [ty] PVar ty
+| typed_abs {n} ty1 gamma (pt : pterm (S n)) ty2 :
+  is_typed (gamma :: ty1) pt ty2 -> is_typed gamma (PAbs pt) (TImp ty1 ty2)
+| typed_app {n m} gamma delta (pt1 : pterm n) (pt2 : pterm m) ty1 ty2:
+  is_typed gamma pt1 (TImp ty1 ty2) -> is_typed delta pt2 ty1 ->
+  is_typed (gamma ++ delta) (PApp pt1 pt2) ty2.
 
-Check test2.
+(* ===== Substitution ===== *)
 
-(*
-Inductive is_typed : context -> pterm (a : nat) -> type -> Prop :=
-| type_var ty : is_typed [ty] PVar ty.
-*)
+Definition s_rule : Type := nat * type.
+Definition s_rules : Type := list s_rule.
+
+Fixpoint subst (rul : s_rule) (ty : type) : type :=
+match ty with
+| TVar n => let (m, u) := rul in
+  match eqb n m with
+  | true => u
+  | false => ty
+  end
+| TImp ty1 ty2 => TImp (subst rul ty1) (subst rul ty2)
+end.
+
+Fixpoint subst_ty (sigma : s_rules) (ty : type) : type :=
+match sigma with
+| List.nil => ty
+| List.cons rul sigma' =>
+  subst_ty sigma' (subst rul ty)
+end.
+
+Fixpoint subst_ctx {n : nat} (sigma : s_rules) (ctx : context n) : context n :=
+match ctx with
+| [] => []
+| ctx' :: ty => (subst_ctx sigma ctx') :: (subst_ty sigma ty)
+end.
+
+Lemma subst_typed : forall {n : nat} (sigma : s_rules) (ctx : context n) (pt : pterm n) (ty : type),
+  is_typed ctx pt ty -> is_typed (subst_ctx sigma ctx) pt (subst_ty sigma ty).
+Admitted.
+
+Definition is_princ : Type := forall {n : nat} (ctx : context n) (pt : pterm n) (ty : type),
+  is_typed ctx pt ty -> forall (ctx' : context n) (ty' : type), is_typed ctx' pt ty' ->
+  sig (fun (sigma : s_rules) => ctx' = subst_ctx sigma ctx /\ ty' = subst_ty sigma ty).
+
+(* ===== Inference ===== *)
+
+Definition type_eq : Type := type * type.
+Definition constraints : Type := list type_eq.
+
+Definition length {A : Type} {n : nat} : snoclist A n -> nat := fix length l := n.
+
+(*Check let (pair a b, c) := (pair 1 2, 3) in a.*)
+
+Fixpoint Bidir_synth {n : nat} (fresh : nat) (t : pterm n) : (nat * context n * type * constraints) :=
+match t in pterm n return (nat * context n * type * constraints) with
+| PAbs t' =>
+  let (temp, const) := Bidir_synth fresh t' in
+  let (temp', B) := temp in
+  let (fresh', ctx') := temp' in
+  match ctx' in snoclist _ (S n) return (nat * context n * type * constraints) with
+  | ctx'' :: A => (fresh', ctx'', TImp A B, const)
+  end
+| PVar =>
+  let (temp, const) := Bidir_check (S fresh) PVar (TVar fresh) in
+  let (fresh', ctx') := temp in
+  (fresh', ctx', (TVar fresh), const)
+| PApp pt1 pt2 =>
+  let (temp, const) := Bidir_check (S fresh) (PApp pt1 pt2) (TVar fresh) in
+  let (fresh', ctx') := temp in
+  (fresh', ctx', (TVar fresh), const)
+end
+
+with Bidir_check {n : nat} (fresh : nat) (t : pterm n) : type -> (nat * context n * constraints) :=
+fix Bidir_check fresh t ty :=
+match t in pterm n return (nat * context n * constraints) with
+| PVar => (fresh, [ty], List.nil)
+| PApp pt1 pt2 =>
+  let (temp, const2) := Bidir_synth fresh pt2 in
+  let (temp', A) := temp in
+  let (fresh', ctx2) := temp' in
+  let (temp, const1) := Bidir_check fresh' pt1 (TImp A ty) in
+  let (fresh'', ctx1) := temp' in
+  (fresh'', ctx1 ++ ctx2, List.app const1 const2)
+| PAbs t' =>
+  let (temp, const) := Bidir_synth fresh (PAbs t') in
+  let (temp', A) := temp in
+  let (fresh', ctx') := temp' in
+  (fresh', ctx', List.cons (A, ty) const)
+end.
+
+
+
+
+
+
+
+
+
+
+
+
+
+
