README.txt
@@ -1,0 +1,21 @@
+build:
+
+coq_makefile -f _CoqProject -o CoqMakeFile
+make -f CoqMakeFile
+
+clean:
+
+make -f CoqMakeFile clean
+
+- substitution
+- type substitution
+- proof of subst_typed
+- change bidir into a predicate
+- add shape-annotated planar lambda-terms
+- do shape annotated bidir
+- some predicate on the principal typing
+- sigma satisfies constraints
+
+G <= t => A　｜三 ->
+s |= 三 ->
+sG |- t : sA
